src/Platform/Minimal.v
@@ -149,18 +149,12 @@ Section Riscv.
        | |- _ \/ _ => right; solve [t]
        end.
 
-  Instance MinimalPrimitivesParams: PrimitivesParams (OState RiscvMachine) RiscvMachine := {|
+  Instance MinimalPrimitivesParams: PrimitivesParams (OState RiscvMachine) RiscvMachine := {
     Primitives.mcomp_sat := @OStateOperations.computation_with_answer_satisfies RiscvMachine;
     Primitives.is_initial_register_value := eq (word.of_Z 0);
-    Primitives.nonmem_loadByte_sat   initialL addr post := False;
-    Primitives.nonmem_loadHalf_sat   initialL addr post := False;
-    Primitives.nonmem_loadWord_sat   initialL addr post := False;
-    Primitives.nonmem_loadDouble_sat initialL addr post := False;
-    Primitives.nonmem_storeByte_sat   initialL addr v post := False;
-    Primitives.nonmem_storeHalf_sat   initialL addr v post := False;
-    Primitives.nonmem_storeWord_sat   initialL addr v post := False;
-    Primitives.nonmem_storeDouble_sat initialL addr v post := False;
-  |}.
+    Primitives.nonmem_load n addr := fail_hard;
+    Primitives.nonmem_store n addr v := fail_hard;
+  }.
 
   Instance MinimalSatisfiesPrimitives: Primitives MinimalPrimitivesParams.
   Proof.
